theories/MinskyMachines/MM/mm_comp_strong.v
@@ -1,0 +1,270 @@
+(**************************************************************)
+(*   Copyright Dominique Larchey-Wendling [*]                 *)
+(*                                                            *)
+(*                             [*] Affiliation LORIA -- CNRS  *)
+(**************************************************************)
+(*      This file is distributed under the terms of the       *)
+(*         CeCILL v2 FREE SOFTWARE LICENSE AGREEMENT          *)
+(**************************************************************)
+
+Require Import List Arith Lia.
+
+From Undecidability.Shared.Libs.DLW 
+  Require Import utils list_bool pos vec
+                 subcode sss compiler_correction.
+
+From Undecidability.StackMachines.BSM
+  Require Import bsm_defs.
+
+From Undecidability.MinskyMachines.MM
+  Require Import mm_defs mm_utils. 
+
+Set Implicit Arguments.
+
+Set Default Proof Using "Type".
+
+(* ** BSM recues to MM *)
+
+Tactic Notation "rew" "length" := autorewrite with length_db.
+
+Local Notation "e #> x" := (vec_pos e x).
+Local Notation "e [ v / x ]" := (vec_change e x v).
+
+Local Notation "I '/BSM/' s -1> t" := (bsm_sss I s t) (at level 70, no associativity).
+Local Notation "P '/BSM/' s -+> t" := (sss_progress (@bsm_sss _) P s t) (at level 70, no associativity).
+Local Notation "P '/BSM/' s ->> t" := (sss_compute (@bsm_sss _) P s t) (at level 70, no associativity).
+Local Notation "P '/BSM/' s ~~> t" := (sss_output (@bsm_sss _) P s t) (at level 70, no associativity).
+Local Notation "P '/BSM/' s ↓" := (sss_terminates (@bsm_sss _) P s)(at level 70, no associativity).
+
+Local Notation "P '/MM/' s -+> t" := (sss_progress (@mm_sss _) P s t) (at level 70, no associativity).
+Local Notation "P '/MM/' s ->> t" := (sss_compute (@mm_sss _) P s t) (at level 70, no associativity).
+Local Notation "P '/MM/' s '~~>' t" := (sss_output (@mm_sss _) P s t) (at level 70, no associativity).
+Local Notation "P '/MM/' s ↓" := (sss_terminates (@mm_sss _) P s)(at level 70, no associativity).
+
+Section simulator.
+
+  Ltac dest x y := destruct (pos_eq_dec x y) as [ | ]; [ subst x | ]; rew vec.
+
+  Variables (m : nat).
+  
+  (* each stack of the BSM corresponds to a (unique) register in the MM 
+      and there are extra registers: tmp1, tmp2 which must have value 0 at start 
+      they might change value during a simulated BSM instruction but when
+      the instruction is finished, their values are back to 0 
+
+      This is expressed in the below bsm_state_enc invariant
+  *)
+  
+  Let n := m + 2.
+  Variable tmp1 : pos n. 
+  Variable tmp2 : pos n.
+  Variable reg : pos m -> pos n.
+   
+  Hypothesis Hv12 : tmp1 <> tmp2.
+  Hypothesis Hvr1 : forall p, reg p <> tmp1. 
+  Hypothesis Hvr2 : forall p, reg p <> tmp2.
+  
+  Hypothesis Hreg : forall p q, reg p = reg q -> p = q.
+
+  Variable cases : forall p : pos n, {p = tmp1} + {p = tmp2} + {q | p = reg q}.
+
+  Definition bsm_state_enc (v : vec (list bool) m) w := 
+            w#>tmp1 = 0
+         /\ w#>tmp2 = 0
+         /\ forall p, w#>(reg p) = stack_enc (v#>p).
+
+  (* i is the position in the source code *)
+
+  Definition bsm_instr_compile lnk i ii :=
+    match ii with
+      | PUSH s Zero => mm_push_Zero (reg s) tmp1 tmp2 (lnk i)
+      | PUSH s One  => mm_push_One  (reg s) tmp1 tmp2 (lnk i)
+      | POP  s j k  => mm_pop (reg s) tmp1 tmp2 (lnk i) (lnk j) (lnk (1+i)) (lnk k)
+    end.
+
+  Definition bsm_instr_compile_length (ii : bsm_instr m) :=
+    match ii with 
+      | PUSH _ Zero => 7
+      | PUSH _ One  => 8
+      | POP  _ _ _  => 16
+    end.
+
+  Fact bsm_instr_compile_length_eq lnk i ii : length (bsm_instr_compile lnk i ii) = bsm_instr_compile_length ii.
+  Proof. destruct ii as [ | ? [] ]; simpl; auto. Qed.
+    
+  Fact bsm_instr_compile_length_geq ii : 1 <= bsm_instr_compile_length ii.
+  Proof. destruct ii as [ | ? [] ]; simpl; auto; lia. Qed.
+
+  Hint Resolve bsm_instr_compile_length_eq bsm_instr_compile_length_geq : core.
+
+  (* This main soundness lemma per simulated instruction *)
+
+  Lemma bsm_instr_compile_sound : instruction_compiler_sound bsm_instr_compile (@bsm_sss _) (@mm_sss _) bsm_state_enc.
+  Proof using Hvr1 Hvr2 Hv12 Hreg.
+    intros lnk I i1 v1 i2 v2 w1 H; revert H w1.
+    change v1 with (snd (i1,v1)) at 2.
+    change i1 with (fst (i1,v1)) at 2 3 4 6 7 8.
+    change v2 with (snd (i2,v2)) at 2.
+    change i2 with (fst (i2,v2)) at 2.
+    generalize (i1,v1) (i2,v2); clear i1 v1 i2 v2.
+    induction 1 as    [ i p j k v Hv
+                      | i p j k v ll Hll 
+                      | i p j k v ll Hll
+                      | i p [] v
+                      ]; simpl; intros w1 H0 H; generalize H; intros (H1 & H2 & H3).
+
+    + exists w1; split; auto.
+      apply mm_pop_void_progress; auto using Hv12, Hvr1, Hvr2.
+      rewrite H3, Hv; auto.
+
+    + exists (w1[(stack_enc ll)/reg p]); repeat split; auto; rew vec.
+      * apply mm_pop_Zero_progress; auto using Hv12, Hvr1, Hvr2.
+        rewrite H3, Hll; auto.
+      * rewrite vec_change_neq. 2: congruence. eauto. 
+      * rewrite vec_change_neq. 2: congruence. eauto. 
+      * intros q; dest p q.
+        assert (reg p <> reg q); rew vec.
+    
+    + exists (w1[(stack_enc ll)/reg p]); repeat split; auto; rew vec.
+      * apply mm_pop_One_progress; auto using Hv12, Hvr1, Hvr2.
+        rewrite H3, Hll; auto.
+      * rewrite vec_change_neq. 2: congruence. eauto. 
+      * rewrite vec_change_neq. 2: congruence. eauto. 
+      * intros q; dest p q.
+        assert (reg p <> reg q); rew vec.
+   
+    + exists (w1[(stack_enc (One::v#>p))/reg p]); repeat split; auto; rew vec.
+      2:{ rewrite vec_change_neq. 2: congruence. eauto. } 
+      2:{ rewrite vec_change_neq. 2: congruence. eauto. }
+      rewrite H0; apply mm_push_One_progress; auto using Hv12, Hvr1, Hvr2.
+      intros q; dest p q.
+      assert (reg p <> reg q); rew vec.
+
+    + exists (w1[(stack_enc (Zero::v#>p))/reg p]); repeat split; auto; rew vec.
+      rewrite H0; apply mm_push_Zero_progress; auto using Hv12, Hvr1, Hvr2.
+      * rewrite vec_change_neq. 2: congruence. eauto. 
+      * rewrite vec_change_neq. 2: congruence. eauto. 
+      * intros q; dest p q.
+        assert (reg p <> reg q); rew vec.
+  Qed.
+
+  Hint Resolve bsm_instr_compile_sound : core.
+
+  Section bsm_sim.
+
+    Variable (iP : nat) (cP : list (bsm_instr m)) (iQ : nat).
+
+    Local Definition lnk_Q_pair := @gen_compiler_correction _ _ _ _ bsm_instr_compile_length_eq _ _ _ _  (@bsm_sss_total' _)
+                     (@mm_sss_fun _) _ bsm_instr_compile_sound (iP,cP) iQ. 
+
+    Local Definition lnk := projT1 lnk_Q_pair.
+    Local Definition Q := proj1_sig (projT2 lnk_Q_pair).
+    
+    Local Lemma code_endQ : code_end Q = iQ + length (snd Q).
+    Proof.
+      unfold Q, lnk_Q_pair. cbn.
+      f_equal. now destruct gen_compiler_correction as (? & ? & ? & ?); cbn.
+    Qed.
+
+    Local Lemma Hlnk : fst Q = iQ /\ lnk iP = iQ /\ forall i, out_code i (iP,cP) -> lnk i = code_end Q.
+    Proof.
+      repeat split; apply (proj2_sig (projT2 lnk_Q_pair)).
+    Qed.
+
+    Infix "⋈" := bsm_state_enc (at level 70, no associativity).
+
+    Local Lemma HQ1 : forall i1 v1 w1 i2 v2, v1 ⋈ w1 /\ (iP,cP) /BSM/ (i1,v1) ~~> (i2,v2)     
+                    -> exists w2,    v2 ⋈ w2 /\ Q /MM/ (lnk i1,w1) ~~> (lnk i2,w2).
+    Proof. apply (proj2_sig (projT2 lnk_Q_pair)). Qed.
+
+    Local Lemma HQ2 : forall i1 v1 w1 j2 w2, v1 ⋈ w1 /\ Q /MM/ (lnk i1,w1) ~~> (j2,w2) 
+                    -> exists i2 v2, v2 ⋈ w2 /\ (iP,cP) /BSM/ (i1,v1) ~~> (i2,v2) /\ j2 = lnk i2.
+    Proof. apply (proj2_sig (projT2 lnk_Q_pair)). Qed.
+
+    Variable v : vec (list bool) m. 
+
+    Definition vec_enc v := vec_set_pos (fun p => match cases p with inl _ => 0 | inr (exist _ q _) => (stack_enc (v#>q)) end).
+
+    Local Definition w := vec_enc v.
+
+    Let vec_enc_spec : forall v, bsm_state_enc v (vec_enc v).
+    Proof.
+      red; unfold vec_enc; repeat split; rew vec.
+      - destruct (cases tmp1) as [[ | ] | [q Hq]]; try firstorder congruence.
+      - destruct (cases tmp2) as [[ | ] | [q Hq]]; try firstorder congruence.
+      - intros p. rewrite vec_pos_set.  destruct (cases (reg p)) as [[ | ] | [q Hq]]; try now firstorder congruence.
+    Qed.
+
+    Let w_prop : bsm_state_enc v w.
+    Proof.
+      eapply vec_enc_spec.
+    Qed.
+
+    (* (iQ,cQ) simulates termination of (iP,cP) while ensuring tmp1 and tmp2 stay void when it terminates *)
+
+    Local Lemma Q_spec1 : (iP,cP) /BSM/ (iP,v) ↓ -> exists w', Q /MM/ (iQ,w) ~~> (code_end Q, w') /\ w'#>tmp1 = 0 /\ w'#>tmp2 = 0.
+    Proof.
+      intros ((i1,v1) & H1).
+      destruct HQ1 with (1 := conj w_prop H1) as (w' & H2 & H3).
+      rewrite <- (proj2 (proj2 Hlnk) i1), <- (proj1 (proj2 Hlnk)).
+      * exists w'; split; auto; red in H2; tauto.
+      * apply H1.
+    Qed.
+
+    Local Lemma Q_spec1_strong i1 v1 : (iP,cP) /BSM/ (iP,v) ~~> (i1, v1) -> Q /MM/ (iQ,w) ~~> (code_end Q, vec_enc v1).
+    Proof.
+      intros H1.
+      destruct HQ1 with (1 := conj w_prop H1) as (w' & H2 & H3).
+      rewrite <- (proj2 (proj2 Hlnk) i1), <- (proj1 (proj2 Hlnk)).
+      * eenough (w' = vec_enc v1) as <- by eassumption.
+        destruct H2 as (H2 & H4 & H5).
+        eapply vec_pos_ext. intros p. unfold vec_enc. rewrite vec_pos_set.
+        destruct (cases p) as [[E | E ] | [q E]]; subst; rew vec.
+      * apply H1.
+    Qed.    
+
+    Local Lemma Q_spec2 : Q /MM/ (iQ,w) ↓ -> (iP,cP) /BSM/ (iP,v) ↓.
+    Proof.
+      intros ((j,w2) & H1).
+      rewrite <- (proj1 (proj2 Hlnk)) in H1.
+      destruct HQ2 with (1 := conj w_prop H1) as (i2 & v2 & H2 & H3 & _).
+      exists (i2,v2); auto.
+    Qed.
+
+    Definition bsm_mm_sim := snd Q.
+
+    Theorem bsm_mm_sim_spec : (iP,cP) /BSM/ (iP,v) ↓ <-> (iQ,bsm_mm_sim) /MM/ (iQ,w) ↓.
+    Proof.
+      rewrite <- (proj1 Hlnk) at 1.
+      rewrite <- surjective_pairing.
+      split; auto using Q_spec2.
+      intros H.
+      destruct (Q_spec1 H) as (w' & H1 & _).
+      exists (code_end Q, w'); auto.
+    Qed.
+
+    Theorem bsm_mm_sim_spec_strong i1 v1 : (iP,cP) /BSM/ (iP,v) ~~> (i1, v1) -> (iQ,bsm_mm_sim) /MM/ (iQ,w) ~~> (iQ + length bsm_mm_sim, vec_enc v1).
+    Proof.
+      rewrite <- (proj1 Hlnk) at 1.
+      rewrite <- surjective_pairing.
+      unfold bsm_mm_sim. rewrite <- code_endQ.
+      apply Q_spec1_strong.
+    Qed.
+
+    End bsm_sim.
+
+End simulator.
+
+Theorem bsm_mm_compiler_strong n i (P : list (bsm_instr n)) (tmp1 tmp2 : pos (n + 2)) (reg : pos n -> pos (n + 2)) iQ :
+  tmp1 <> tmp2 -> (forall p, tmp1 <> reg p) -> (forall p, tmp2 <> reg p) -> (forall p q, reg p = reg q -> p = q) ->
+  forall cases : (forall p : pos _, {p = tmp1} + {p = tmp2} + {q | p = reg q}),
+  { Q : list (mm_instr (pos (n+2))) | (forall v, (i,P) /BSM/ (i,v) ↓ <-> (iQ,Q) /MM/ (iQ,(@vec_enc _ tmp1 tmp2 reg cases v)) ↓) /\
+                                      forall v j w, (i,P) /BSM/ (i,v) ~~> (j,w) -> (iQ,Q) /MM/ (iQ, @vec_enc _ tmp1 tmp2 reg cases v) ~~> (iQ + length Q, @vec_enc _ tmp1 tmp2 reg cases w) }.
+Proof. 
+  intros.    
+  unshelve eexists (@bsm_mm_sim _ tmp1 tmp2 reg _ _ _ _ i P _); eauto.
+  split.
+  - apply bsm_mm_sim_spec.
+  - intros. match goal with [ |- context[ iQ + length ?Q ]] => change (iQ + length Q) with (code_end (iQ, Q)) end.
+    eapply bsm_mm_sim_spec_strong; eauto.
+Qed.
